theories/interop/update_laws.v
@@ -67,7 +67,7 @@ Lemma freeze_foreign_to_immut γ θ b :
     GC θ ∗ γ ↦foreign[Immut] b.
 Proof.
   iIntros "(HGC & [Hγ1 Hγ2])". iNamed "HGC".
-  assert (freeze_block (Bforeign Mut (Some b)) (Bforeign Immut (Some b))) as Hfreeze.
+  assert (freeze_block (Bforeign (Mut, Some b)) (Bforeign (Immut, Some b))) as Hfreeze.
     { econstructor. }
   iMod (hgh_freeze_block _ _ _ _ _ _ Hfreeze with "GCHGH Hγ1 Hγ2") as "(GCHGH & Hmtζ & Hmtfresh)".
   iModIntro. iSplitR "Hmtζ Hmtfresh"; last by iFrame; eauto.
